plugin/evaluation.ml
@@ -1,7 +1,8 @@
-(** This file reifies level zero terms/substitutions into level one terms/substitutions.
+(** This file evaluates level one terms/substitutions into level zero terms/substitutions.
 *)
 
 open Prelude
+module C = Constants
 
 module Make (P : sig
   val sign : signature
@@ -17,20 +18,48 @@ struct
   (** *** Patterns. *)
   (**************************************************************************************)
 
+  let is_glob' (env : Environ.env) (sigma : Evd.evar_map) (name : Names.GlobRef.t Lazy.t)
+      (t : EConstr.t) : bool =
+    is_glob env sigma (Lazy.force name) t
+
   (** Pattern which matches [O.E_Var ?i]. *)
   let var_patt : EConstr.t patt =
    fun t env sigma ->
+    (*match EConstr.kind sigma t with
+    | App (f, [| _; i |]) -> begin
+        match EConstr.kind sigma f with
+        | Construct (c, _) ->
+            Log.printf "var_patt: %s =can= %s := %b"
+              (Pp.string_of_ppcmds @@ Names.GlobRef.print @@ Names.GlobRef.ConstructRef c)
+              (Pp.string_of_ppcmds @@ Names.GlobRef.print @@ Lazy.force C.O.e_var)
+              (Names.GlobRef.CanOrd.equal (Names.GlobRef.ConstructRef c)
+                 (Lazy.force C.O.e_var));
+            Log.printf "var_patt: %s =user= %s := %b"
+              (Pp.string_of_ppcmds @@ Names.GlobRef.print @@ Names.GlobRef.ConstructRef c)
+              (Pp.string_of_ppcmds @@ Names.GlobRef.print @@ Lazy.force C.O.e_var)
+              (Names.GlobRef.UserOrd.equal (Names.GlobRef.ConstructRef c)
+                 (Lazy.force C.O.e_var));
+            Log.printf "var_patt: %s =syntactic= %s := %b"
+              (Pp.string_of_ppcmds @@ Names.GlobRef.print @@ Names.GlobRef.ConstructRef c)
+              (Pp.string_of_ppcmds @@ Names.GlobRef.print @@ Lazy.force C.O.e_var)
+              (Names.GlobRef.SyntacticOrd.equal (Names.GlobRef.ConstructRef c)
+                 (Lazy.force C.O.e_var));
+            (sigma, None)
+        | _ -> (sigma, None)
+      end
+    | _ -> (sigma, None)*)
     match EConstr.kind sigma t with
-    | App (f, [| i |]) when is_ctor sigma P.ops1.e_var f -> (sigma, Some i)
+    | App (f, [| _; i |]) when is_glob' env sigma C.O.e_var f -> (sigma, Some i)
     | _ -> (sigma, None)
 
   (** Pattern which matches a single argument of type [ty]. *)
   let rec arg_patt (ty : arg_ty) : EConstr.t patt =
    fun a env sigma ->
     match (ty, EConstr.kind sigma a) with
-    | AT_base _, App (f, [| _; x |]) when is_ctor sigma P.ops1.e_abase f -> (sigma, Some x)
-    | AT_term, App (f, [| t |]) when is_ctor sigma P.ops1.e_aterm f -> (sigma, Some t)
-    | AT_bind ty, App (f, [| _; a |]) when is_ctor sigma P.ops1.e_abind f ->
+    | AT_base _, App (f, [| _; _; x |]) when is_glob' env sigma C.O.e_abase f ->
+        (sigma, Some x)
+    | AT_term, App (f, [| _; t |]) when is_glob' env sigma C.O.e_aterm f -> (sigma, Some t)
+    | AT_bind ty, App (f, [| _; _; a |]) when is_glob' env sigma C.O.e_abind f ->
         arg_patt ty a env sigma
     | _ -> (sigma, None)
 
@@ -38,8 +67,9 @@ struct
   let rec args_patt (tys : arg_ty list) : EConstr.t list patt =
    fun al env sigma ->
     match (tys, EConstr.kind sigma al) with
-    | [], _ when is_ctor sigma P.ops1.e_al_nil al -> (sigma, Some [])
-    | ty :: tys, App (f, [| _; _; a; al |]) when is_ctor sigma P.ops1.e_al_cons f -> begin
+    | [], App (f, [| _ |]) when is_glob' env sigma C.O.e_al_nil f -> (sigma, Some [])
+    | ty :: tys, App (f, [| _; _; _; a; al |]) when is_glob' env sigma C.O.e_al_cons f ->
+      begin
         match arg_patt ty a env sigma with
         | sigma, None -> (sigma, None)
         | sigma, Some a -> begin
@@ -54,7 +84,7 @@ struct
   let ctor_patt : (int * EConstr.t list) patt =
    fun t env sigma ->
     match EConstr.kind sigma t with
-    | App (f, [| c; al |]) when is_ctor sigma P.ops1.e_ctor f -> begin
+    | App (f, [| _; c; al |]) when is_glob' env sigma C.O.e_ctor f -> begin
         match EConstr.kind sigma c with
         | Construct ((ctor, i), _) when Names.Ind.UserOrd.equal ctor P.ops1.ctor -> begin
             let tys = P.sign.ctor_types.(i - 1) in
@@ -70,14 +100,15 @@ struct
   let rename_patt : (EConstr.t * EConstr.t) patt =
    fun t env sigma ->
     match EConstr.kind sigma t with
-    | App (f, [| _; r; t |]) when is_const sigma P.ops1.rename f -> (sigma, Some (r, t))
+    | App (f, [| _; _; r; t |]) when is_glob' env sigma C.O.rename f ->
+        (sigma, Some (r, t))
     | _ -> (sigma, None)
 
   (** Pattern which matches [O.substitute ?s ?t]. *)
   let substitute_patt : (EConstr.t * EConstr.t) patt =
    fun t env sigma ->
     match EConstr.kind sigma t with
-    | App (f, [| _; s; t |]) when is_const sigma P.ops1.substitute f ->
+    | App (f, [| _; _; s; t |]) when is_glob' env sigma C.O.substitute f ->
         (sigma, Some (s, t))
     | _ -> (sigma, None)
 
@@ -85,57 +116,64 @@ struct
   let reify_patt : EConstr.t patt =
    fun t env sigma ->
     match EConstr.kind sigma t with
-    | App (f, [| t |]) when is_const sigma P.re.reify f -> (sigma, Some t)
+    | App (f, [| t |]) when is_const env sigma P.re.reify f -> (sigma, Some t)
     | _ -> (sigma, None)
 
   (** Pattern which matches [O.sid]. *)
   let sid_patt : unit patt =
    fun s env sigma ->
-    if is_const sigma P.ops1.sid s then (sigma, Some ()) else (sigma, None)
+    match EConstr.kind sigma s with
+    | App (f, [| _ |]) when is_glob' env sigma C.O.sid f -> (sigma, Some ())
+    | _ -> (sigma, None)
 
   (** Pattern which matches [O.sshift]. *)
   let sshift_patt : unit patt =
    fun s env sigma ->
-    if is_const sigma P.ops1.sshift s then (sigma, Some ()) else (sigma, None)
+    match EConstr.kind sigma s with
+    | App (f, [| _ |]) when is_glob' env sigma C.O.sshift f -> (sigma, Some ())
+    | _ -> (sigma, None)
 
   (** Pattern which matches [O.scons ?t ?s]. *)
   let scons_patt : (EConstr.t * EConstr.t) patt =
    fun s env sigma ->
     match EConstr.kind sigma s with
-    | App (f, [| t; s |]) when is_const sigma P.ops1.scons f -> (sigma, Some (t, s))
+    | App (f, [| _; t; s |]) when is_glob' env sigma C.O.scons f -> (sigma, Some (t, s))
     | _ -> (sigma, None)
 
   (** Pattern which matches [O.scomp ?s1 ?s2]. *)
   let scomp_patt : (EConstr.t * EConstr.t) patt =
    fun s env sigma ->
     match EConstr.kind sigma s with
-    | App (f, [| s1; s2 |]) when is_const sigma P.ops1.scomp f -> (sigma, Some (s1, s2))
+    | App (f, [| _; s1; s2 |]) when is_glob' env sigma C.O.scomp f ->
+        (sigma, Some (s1, s2))
     | _ -> (sigma, None)
 
   (** Pattern which matches [O.rscomp ?r ?s]. *)
   let rscomp_patt : (EConstr.t * EConstr.t) patt =
    fun s env sigma ->
     match EConstr.kind sigma s with
-    | App (f, [| r; s |]) when is_const sigma P.ops1.rscomp f -> (sigma, Some (r, s))
+    | App (f, [| _; r; s |]) when is_glob' env sigma C.O.rscomp f -> (sigma, Some (r, s))
     | _ -> (sigma, None)
 
   (** Pattern which matches [O.srcomp ?s ?r]. *)
   let srcomp_patt : (EConstr.t * EConstr.t) patt =
    fun s env sigma ->
     match EConstr.kind sigma s with
-    | App (f, [| s; r |]) when is_const sigma P.ops1.srcomp f -> (sigma, Some (s, r))
+    | App (f, [| _; s; r |]) when is_glob' env sigma C.O.srcomp f -> (sigma, Some (s, r))
     | _ -> (sigma, None)
 
   (** Pattern which matches [O.E_var]. *)
   let var_patt_no_args : unit patt =
-   fun s env sigma ->
-    if is_ctor sigma P.ops1.e_var s then (sigma, Some ()) else (sigma, None)
+   fun t env sigma ->
+    match EConstr.kind sigma t with
+    | App (f, [| _ |]) when is_glob' env sigma C.O.e_var f -> (sigma, Some ())
+    | _ -> (sigma, None)
 
   (** Pattern which matches [O.sreify ?s]. *)
   let sreify_patt : EConstr.t patt =
    fun s env sigma ->
     match EConstr.kind sigma s with
-    | App (f, [| s |]) when is_const sigma P.re.sreify f -> (sigma, Some s)
+    | App (f, [| s |]) when is_const env sigma P.re.sreify f -> (sigma, Some s)
     | _ -> (sigma, None)
 
   (**************************************************************************************)
@@ -146,7 +184,7 @@ struct
     (* Branch for [O.E_Var ?i]. *)
     let var_branch i =
       let t = app (mkctor (P.ops0.term, 1)) i in
-      let* p = apps_ev (Lazy.force Consts.eq_refl) 1 [| t |] in
+      let* p = apps_ev (mkglob' C.eq_refl) 1 [| t |] in
       ret (t, p)
     in
     (* Branch for [O.E_ctor ?c ?al]. *)
@@ -154,7 +192,7 @@ struct
       let rec eval_arg ty a : (EConstr.t * EConstr.t) m =
         match ty with
         | AT_base _ ->
-            let* p = apps_ev (Lazy.force Consts.eq_refl) 1 [| a |] in
+            let* p = apps_ev (mkglob' C.eq_refl) 1 [| a |] in
             ret (a, p)
         | AT_term -> eval_term a
         | AT_bind ty -> eval_arg ty a
@@ -170,12 +208,12 @@ struct
     in
     (* Branch for [O.rename ?r ?t1']. *)
     let rename_branch (r, t1') =
-      let* p_r = apps_ev (Lazy.force Consts.reflexivity) 3 [| r |] in
+      let* p_r = apps_ev (mkglob' C.reflexivity) 3 [| r |] in
       let* t1, p_t1 = eval_term t1' in
       let t = apps (mkconst P.ops0.rename) [| r; t1 |] in
       let p1 = apps (mkconst P.pe.eval_rename) [| r; t1' |] in
       let* p2 = apps_ev (mkconst P.congr.congr_rename) 4 [| p_r; p_t1 |] in
-      let* p = apps_ev (Lazy.force Consts.transitivity) 6 [| p1; p2 |] in
+      let* p = apps_ev (mkglob' C.transitivity) 6 [| p1; p2 |] in
       ret (t, p)
     in
     (* Branch for [O.substitute ?s' ?t1']. *)
@@ -185,7 +223,7 @@ struct
       let t = apps (mkconst P.ops0.substitute) [| s; t1 |] in
       let p1 = apps (mkconst P.pe.eval_substitute) [| s'; t1' |] in
       let* p2 = apps_ev (mkconst P.congr.congr_substitute) 4 [| p_s; p_t1 |] in
-      let* p = apps_ev (Lazy.force Consts.transitivity) 6 [| p1; p2 |] in
+      let* p = apps_ev (mkglob' C.transitivity) 6 [| p1; p2 |] in
       ret (t, p)
     in
     (* Branch for [reify ?t]. *)
@@ -193,7 +231,7 @@ struct
     (* Default branch. *)
     let default_branch t' =
       let t = apps (mkconst P.re.eval) [| kt P.ops1; t' |] in
-      let* p = apps_ev (Lazy.force Consts.eq_refl) 1 [| t |] in
+      let* p = apps_ev (mkglob' C.eq_refl) 1 [| t |] in
       ret (t, p)
     in
     (* Actual pattern matching. *)
@@ -210,13 +248,13 @@ struct
     (* Match [O.sid]. *)
     let sid_branch () =
       let s = mkconst P.ops0.sid in
-      let* p = apps_ev (Lazy.force Consts.reflexivity) 3 [| s |] in
+      let* p = apps_ev (mkglob' C.reflexivity) 3 [| s |] in
       ret (s, p)
     in
     (* Match [O.sshift]. *)
     let sshift_branch () =
       let s = mkconst P.ops0.sshift in
-      let* p = apps_ev (Lazy.force Consts.reflexivity) 3 [| s |] in
+      let* p = apps_ev (mkglob' C.reflexivity) 3 [| s |] in
       ret (s, p)
     in
     (* Match [O.scons ?t' ?s1']. *)
@@ -226,7 +264,7 @@ struct
       let s = apps (mkconst P.ops0.scons) [| t; s1 |] in
       let p1 = apps (mkconst P.pe.seval_scons) [| t'; s1' |] in
       let* p2 = apps_ev (mkconst P.congr.congr_scons) 4 [| p_t; p_s1 |] in
-      let* p = apps_ev (Lazy.force Consts.transitivity) 6 [| p1; p2 |] in
+      let* p = apps_ev (mkglob' C.transitivity) 6 [| p1; p2 |] in
       ret (s, p)
     in
     (* Match [O.scomp ?s1' ?s2']. *)
@@ -236,33 +274,33 @@ struct
       let s = apps (mkconst P.ops0.scomp) [| s1; s2 |] in
       let p1 = apps (mkconst P.pe.seval_scomp) [| s1'; s2' |] in
       let* p2 = apps_ev (mkconst P.congr.congr_scomp) 4 [| p_s1; p_s2 |] in
-      let* p = apps_ev (Lazy.force Consts.transitivity) 6 [| p1; p2 |] in
+      let* p = apps_ev (mkglob' C.transitivity) 6 [| p1; p2 |] in
       ret (s, p)
     in
     (* Match [O.rscomp ?r ?s2']. *)
     let rscomp_branch (r, s2') =
-      let* p_r = apps_ev (Lazy.force Consts.reflexivity) 3 [| r |] in
+      let* p_r = apps_ev (mkglob' C.reflexivity) 3 [| r |] in
       let* s2, p_s2 = eval_subst s2' in
       let s = apps (mkconst P.ops0.rscomp) [| r; s2 |] in
       let p1 = apps (mkconst P.pe.seval_rscomp) [| r; s2' |] in
       let* p2 = apps_ev (mkconst P.congr.congr_rscomp) 4 [| p_r; p_s2 |] in
-      let* p = apps_ev (Lazy.force Consts.transitivity) 6 [| p1; p2 |] in
+      let* p = apps_ev (mkglob' C.transitivity) 6 [| p1; p2 |] in
       ret (s, p)
     in
     (* Match [O.srcomp ?s1' ?r]. *)
     let srcomp_branch (s1', r) =
       let* s1, p_s1 = eval_subst s1' in
-      let* p_r = apps_ev (Lazy.force Consts.reflexivity) 3 [| r |] in
+      let* p_r = apps_ev (mkglob' C.reflexivity) 3 [| r |] in
       let s = apps (mkconst P.ops0.srcomp) [| s1; r |] in
       let p1 = apps (mkconst P.pe.seval_srcomp) [| s1'; r |] in
       let* p2 = apps_ev (mkconst P.congr.congr_srcomp) 4 [| p_s1; p_r |] in
-      let* p = apps_ev (Lazy.force Consts.transitivity) 6 [| p1; p2 |] in
+      let* p = apps_ev (mkglob' C.transitivity) 6 [| p1; p2 |] in
       ret (s, p)
     in
     (* Match [O.E_var]. *)
     let var_branch () =
       let s = mkctor (P.ops0.term, 1) in
-      let* p = apps_ev (Lazy.force Consts.reflexivity) 4 [||] in
+      let* p = apps_ev (mkglob' C.reflexivity) 4 [||] in
       ret (s, p)
     in
     (* Match [sreify ?s]. *)
@@ -270,7 +308,7 @@ struct
     (* Default branch. *)
     let default_branch s' =
       let s = app (mkconst P.re.seval) s' in
-      let* p = apps_ev (Lazy.force Consts.reflexivity) 3 [| s |] in
+      let* p = apps_ev (mkglob' C.reflexivity) 3 [| s |] in
       ret (s, p)
     in
     (* Actual pattern matching. *)
@@ -309,7 +347,7 @@ let eval_term (sign : signature) (ops : ops_all) (t' : EConstr.t) :
   (* Typecheck to resolve evars. *)
   let* _ = typecheck t None in
   let p_ty =
-    apps (Lazy.force Consts.eq)
+    apps (mkglob' C.eq)
       [| mkind ops.ops_ops0.term
        ; apps (mkconst ops.ops_re.eval) [| kt ops.ops_ops1; t' |]
        ; t
@@ -337,12 +375,8 @@ let eval_subst (sign : signature) (ops : ops_all) (s' : EConstr.t) :
   (* Typecheck to resolve evars. *)
   let* _ = typecheck s None in
   let p_ty =
-    apps (Lazy.force Consts.point_eq)
-      [| Lazy.force Consts.nat
-       ; mkind ops.ops_ops0.term
-       ; app (mkconst ops.ops_re.seval) s'
-       ; s
-      |]
+    apps (mkglob' C.point_eq)
+      [| mkglob' C.nat; mkind ops.ops_ops0.term; app (mkconst ops.ops_re.seval) s'; s |]
   in
   let* _ = typecheck p (Some p_ty) in
   ret (s, p)
