plugin/gen_ops_bijection.ml
@@ -1,8 +1,10 @@
 (** This file generates the proof that [eval] and [reify] form a bijection between level
-    zero terms and level one terms. To prove this we also need to generate a custom
-    induction principle on level one terms. *)
+    zero terms and level one terms (actully, currently only one direction is needed). To
+    prove this we also need to generate a custom induction principle on level one terms.
+*)
 
 open Prelude
+module C = Constants
 
 module Make (P : sig
   val sign : signature
@@ -21,19 +23,19 @@ struct
     prod "t" (mkind P.ops0.term) @@ fun t ->
     let t' =
       apps (mkconst P.re.eval)
-        [| app (Lazy.force Consts.k_t) @@ mkind P.ops1.base
+        [| app (mkglob' C.k_t) @@ mkind P.ops1.base
          ; app (mkconst P.re.reify) @@ EConstr.mkVar t
         |]
     in
-    ret @@ apps (Lazy.force Consts.eq) [| mkind P.ops0.term; t'; EConstr.mkVar t |]
+    ret @@ apps (mkglob' C.eq) [| mkind P.ops0.term; t'; EConstr.mkVar t |]
 
   (** Build [forall t, seval (sreify s) =₁ s]. *)
   let build_seval_sreify () : EConstr.t m =
     prod "s" (mkconst P.ops0.subst) @@ fun s ->
     let s' = app (mkconst P.re.seval) @@ app (mkconst P.re.sreify) @@ EConstr.mkVar s in
     ret
-    @@ apps (Lazy.force Consts.point_eq)
-         [| Lazy.force Consts.nat; mkind P.ops0.term; s'; EConstr.mkVar s |]
+    @@ apps (mkglob' C.point_eq)
+         [| mkglob' C.nat; mkind P.ops0.term; s'; EConstr.mkVar s |]
 
   (** Build the induction hypothesis for the non-variable constructor number [idx]
       (starting at [0]). *)
@@ -43,20 +45,22 @@ struct
     let rec build_arg (ty : arg_ty) (arg : Names.Id.t) : EConstr.t m =
       match ty with
       | AT_base b ->
-          ret @@ apps (mkctor P.ops1.e_abase) [| mkctor (P.ops1.base, b + 1); mkVar arg |]
-      | AT_term -> ret @@ apps (mkctor P.ops1.e_aterm) [| mkVar arg |]
+          ret
+          @@ apps (mkglob' C.O.e_abase)
+               [| mkconst P.ops1.sign; mkctor (P.ops1.base, b + 1); mkVar arg |]
+      | AT_term -> ret @@ apps (mkglob' C.O.e_aterm) [| mkconst P.ops1.sign; mkVar arg |]
       | AT_bind ty ->
           let* arg' = build_arg ty arg in
-          apps_ev (mkctor P.ops1.e_abind) 1 [| arg' |]
+          apps_ev (app (mkglob' C.O.e_abind) (mkconst P.ops1.sign)) 1 [| arg' |]
     in
     (* Re-build the list of arguments. *)
     let rec build_args (args : (arg_ty * Names.Id.t) list) : EConstr.t m =
       match args with
-      | [] -> ret @@ mkctor P.ops1.e_al_nil
+      | [] -> ret @@ app (mkglob' C.O.e_al_nil) (mkconst P.ops1.sign)
       | (ty, arg) :: args ->
           let* rarg = build_arg ty arg in
           let* rargs = build_args args in
-          apps_ev (mkctor P.ops1.e_al_cons) 2 [| rarg; rargs |]
+          apps_ev (app (mkglob' C.O.e_al_cons) (mkconst P.ops1.sign)) 2 [| rarg; rargs |]
     in
     (* Build the recursive hypothesis on argument [arg] with arg type [ty].
      Base types ([AT_base]) don't give rise to a hypothesis. *)
@@ -82,43 +86,24 @@ struct
     let* args' = build_args @@ List.combine tys args in
     ret
     @@ app (mkVar pred)
-    @@ apps (mkctor P.ops1.e_ctor) [| mkctor (P.ops1.ctor, idx + 1); args' |]
+    @@ apps (mkglob' C.O.e_ctor)
+         [| mkconst P.ops1.sign; mkctor (P.ops1.ctor, idx + 1); args' |]
 
   (** Build the custom induction principle on level one terms. *)
   let build_ind () : EConstr.t m =
     let open EConstr in
     prod "P" (arrow (term1 P.ops1) mkProp) @@ fun pred ->
     let* var_hyp =
-      prod "i" (Lazy.force Consts.nat) @@ fun i ->
-      ret @@ app (mkVar pred) @@ app (mkctor P.ops1.e_var) @@ mkVar i
+      prod "i" (mkglob' C.nat) @@ fun i ->
+      ret
+      @@ app (mkVar pred)
+      @@ apps (mkglob' C.O.e_var) [| mkconst P.ops1.sign; mkVar i |]
     in
     let* ctor_hyps =
       List.monad_mapi (build_ind_hyp pred) @@ Array.to_list P.sign.ctor_types
     in
     let* concl = prod "t" (term1 P.ops1) @@ fun t -> ret @@ app (mkVar pred) (mkVar t) in
     ret @@ arrows (var_hyp :: ctor_hyps) concl
-
-  (** Build [forall t, reify (eval t) = t]. *)
-  (*let build_reify_eval (ops0 : ops_zero) (ops1 : ops_one) (re : ops_reify_eval) :
-    EConstr.t m =
-  let term1 = app (mkind P.ops1.expr) @@ app (Lazy.force Consts.k_t) @@ mkind P.ops1.base in
-  prod "t" term1 @@ fun t ->
-  let t' =
-    app (mkconst P.re.reify)
-    @@ apps (mkconst P.re.eval)
-         [| app (Lazy.force Consts.k_t) @@ mkind P.ops1.base; EConstr.mkVar t |]
-  in
-  ret @@ apps (Lazy.force Consts.eq) [| term1; t'; EConstr.mkVar t |]
-
-(** Build [forall t, sreify (seval s) =₁ s]. *)
-let build_sreify_seval (ops0 : ops_zero) (ops1 : ops_one) (re : ops_reify_eval) :
-    EConstr.t m =
-  let term1 = app (mkind P.ops1.expr) @@ app (Lazy.force Consts.k_t) @@ mkind P.ops1.base in
-  prod "s" (mkconst P.ops1.subst) @@ fun s ->
-  let s' = app (mkconst P.re.sreify) @@ app (mkconst P.re.seval) @@ EConstr.mkVar s in
-  ret
-  @@ apps (Lazy.force Consts.point_eq)
-       [| Lazy.force Consts.nat; term1; s'; EConstr.mkVar s |]*)
 
   (**************************************************************************************)
   (** *** Prove the lemmas. *)
@@ -162,15 +147,15 @@ let build_sreify_seval (ops0 : ops_zero) (ops1 : ops_one) (re : ops_reify_eval) 
       let* _ = pattern (mkVar arg) in
       match ty with
       | AT_base _ ->
-          let* _ = Tactics.apply (mkconst P.ops1.inv_Ka_base) in
+          let* _ = Tactics.apply (mkglob' C.O.inv_Ka_base) in
           let* _ = intro_fresh "b" in
           ret ()
       | AT_term ->
-          let* _ = Tactics.apply (mkconst P.ops1.inv_Ka_term) in
+          let* _ = Tactics.apply (mkglob' C.O.inv_Ka_term) in
           let* _ = intro_fresh "t" in
           ret ()
       | AT_bind ty' ->
-          let* _ = Tactics.apply (mkconst P.ops1.inv_Ka_bind) in
+          let* _ = Tactics.apply (mkglob' C.O.inv_Ka_bind) in
           let* arg' = intro_fresh "a" in
           inv_arg ty' arg'
     in
@@ -178,9 +163,9 @@ let build_sreify_seval (ops0 : ops_zero) (ops1 : ops_one) (re : ops_reify_eval) 
     let rec inv_args (tys : arg_ty list) (args : Names.Id.t) : unit Proofview.tactic =
       let* _ = pattern (mkVar args) in
       match tys with
-      | [] -> Tactics.apply (mkconst P.ops1.inv_Kal_nil)
+      | [] -> Tactics.apply (mkglob' C.O.inv_Kal_nil)
       | ty :: tys ->
-          let* _ = Tactics.apply (mkconst P.ops1.inv_Kal_cons) in
+          let* _ = Tactics.apply (mkglob' C.O.inv_Kal_cons) in
           let* arg = intro_fresh "a" in
           let* args = intro_fresh "al" in
           inv_arg ty arg >> inv_args tys args
@@ -205,18 +190,19 @@ let build_sreify_seval (ops0 : ops_zero) (ops1 : ops_one) (re : ops_reify_eval) 
     let* ctor_hyps = repeat_n P.sign.n_ctors (intro_fresh "H") in
     (* Apply the well founded induction principle. *)
     let term1 =
-      app (mkind P.ops1.expr) @@ app (Lazy.force Consts.k_t) @@ mkind P.ops1.base
+      apps (mkglob' C.O.expr)
+        [| mkconst P.ops1.sign; app (mkglob' C.k_t) @@ mkind P.ops1.base |]
     in
     let esize =
-      app (mkconst P.ops1.esize) @@ app (Lazy.force Consts.k_t) @@ mkind P.ops1.base
+      apps (mkglob' C.O.esize)
+        [| mkconst P.ops1.sign; app (mkglob' C.k_t) @@ mkind P.ops1.base |]
     in
     let* _ =
-      Tactics.apply
-      @@ apps (Lazy.force Consts.measure_induction) [| term1; esize; mkVar pred |]
+      Tactics.apply @@ apps (mkglob' C.measure_induction) [| term1; esize; mkVar pred |]
     in
     (* Invert [t]. *)
     let* t = intro_fresh "t" in
-    let* _ = pattern (mkVar t) >> Tactics.apply (mkconst P.ops1.inv_Kt) in
+    let* _ = pattern (mkVar t) >> Tactics.apply (mkglob' C.O.inv_Kt) in
     Proofview.tclDISPATCH
       [ (* Solve the [E_var] case. *)
         begin
