plugin/main.ml
@@ -1,5 +1,4 @@
 open Prelude
-open Ltac2_plugin
 
 (* Helper function to build a signature. *)
 let mk_sig (base : EConstr.t list) (ctors : (string * arg_ty list) list) : signature =
@@ -12,13 +11,13 @@ let mk_sig (base : EConstr.t list) (ctors : (string * arg_ty list) list) : signa
 (** A testing signature.*)
 let build_signature () : signature =
   (*mk_sig
-    [ Lazy.force Consts.string ]
+    [ mkglob' Constants.string ]
     [ ("App", [ AT_term; AT_term ]); ("Lam", [ AT_base 0; AT_bind AT_term ]) ]*)
   let level = AT_base 0 in
   let mode = AT_base 1 in
   mk_sig
-    [ Lazy.force @@ Consts.resolve "ghost_reflection.level"
-    ; Lazy.force @@ Consts.resolve "ghost_reflection.mode"
+    [ mkglob' (Constants.resolve "ghost_reflection.level")
+    ; mkglob' (Constants.resolve "ghost_reflection.mode")
     ]
     [ ("Sort", [ mode; level ])
     ; ("Pi", [ level; level; mode; mode; AT_term; AT_bind AT_term ])
@@ -72,13 +71,13 @@ let update_saved_ops : ops_all option -> Libobject.obj =
 
 (** Given a signature, generate all relevant definitions and lemmas (i.e. add them to the
     global environment), and return the names of the generated operations. *)
-let generate_operations (s : signature) : ops_all =
-  let ops0 = Gen_ops_zero.generate s in
-  let ops1 = Gen_ops_one.generate s ops0 in
-  let re = Gen_ops_reify_eval.generate s ops0 ops1 in
-  let congr = Gen_ops_congr.generate s ops0 in
-  let bij = Gen_ops_bijection.generate s ops0 ops1 re congr in
-  let pe = Gen_ops_push_eval.generate s ops0 ops1 re congr bij in
+let generate_operations (sign : signature) : ops_all =
+  let ops0 = Gen_ops_zero.generate sign in
+  let ops1 = Gen_ops_one.generate sign ops0 in
+  let re = Gen_ops_reify_eval.generate sign ops0 ops1 in
+  let congr = Gen_ops_congr.generate sign ops0 in
+  let bij = Gen_ops_bijection.generate sign ops0 ops1 re congr in
+  let pe = Gen_ops_push_eval.generate sign ops0 ops1 re congr bij in
   { ops_ops0 = ops0
   ; ops_ops1 = ops1
   ; ops_re = re
@@ -90,9 +89,9 @@ let generate_operations (s : signature) : ops_all =
 (** Main entry point for the plugin: generate level zero terms, operations, and lemmas. *)
 let generate () =
   (* We use a testing signature (for the moment). *)
-  let s = build_signature () in
+  let sign = build_signature () in
   (* Generate the operations. *)
-  let ops = generate_operations s in
+  let ops = generate_operations sign in
   (* Save the operations. *)
   Lib.add_leaf @@ update_saved_ops (Some ops)
 
@@ -108,6 +107,7 @@ let generate () =
      "name"] *)
 let define_ltac2 (name : string)
     (body : signature -> ops_all -> EConstr.t -> (EConstr.t * EConstr.t) m) : unit =
+  let open Ltac2_plugin in
   let open Tac2externals in
   let open Tac2ffi in
   (* We must delay fetching the saved operations [!saved_ops] until the tactic is 
