theories/RASimpl.v
@@ -1,5 +1,10 @@
-From Prototype Require Import Prelude Sig LevelOne LevelTwo LevelTwoSimp LevelTwoClean.
+From Prototype Require Import Prelude Sig Constants.
+From Prototype Require LevelOne LevelTwo LevelTwoClean.
 From Ltac2 Require Import RedFlags Printf.
+
+Module O := LevelOne.
+Module T := LevelTwo.
+Module Clean := LevelTwoClean.
 
 (*********************************************************************************)
 (** *** Load the plugin. *)
@@ -13,17 +18,11 @@ Ltac2 @external eval_term : constr -> constr * constr := "autosubst-experiments.
 Ltac2 @external eval_subst : constr -> constr * constr := "autosubst-experiments.plugin" "eval_subst".
 
 (*********************************************************************************)
-(** *** Instantiate the generic level 1 and level 2 machinery. *)
+(** *** Reduction flags. *)
 (*********************************************************************************)
 
-(** [Make (S)] creates modules: 
-    - [T] with level two expressions/substitutions built on signature [S].
-    - [O] with level one expressions/substitutions built on signature [S]. *)
-Module Make (S : Sig).
-Include LevelTwoClean.Make (S).
-
 (** Reduction flags to unfold all simplification functions (LevelTwoSimp.v). *)
-Ltac2 red_flags_simp () : RedFlags.t := 
+(*Ltac2 red_flags_simp () : RedFlags.t := 
   red_flags:(beta iota delta 
     [esimp ssimp esimp_functional ssimp_functional
      qsimp rsimp qsimp_functional rsimp_functional
@@ -33,32 +32,31 @@ Ltac2 red_flags_simp () : RedFlags.t :=
      substitute_aux scomp_aux sapply_aux sup rup 
      sapply rscomp sapply_functional rscomp_functional
      rapply rcomp rapply_functional rcomp_functional
-     rcomp_aux rapply_aux rcons scons]).
+     rcomp_aux rapply_aux rcons scons]).*)
 
 (** Reduction flags to unfold all cleanup functions (LevelTwoClean.v). *)
 Ltac2 red_flags_clean () : RedFlags.t :=
   red_flags:(beta iota delta 
-    [eclean sclean eclean_functional sclean_functional
-     qclean rclean qclean_functional rclean_functional
-     eclean_ren eclean_subst eclean_subst_clause_1
-     qclean_rapply qclean_rapply_clause_1
-     dest_rshift dest_rshift_clause_2 dest_rshift_clause_2_clause_1
-     mk_qsucc dest_var
-     dest_ren dest_ren_clause_3 dest_ren_clause_3_clause_1 
-     dest_ren_clause_4 dest_ren_clause_4_clause_1
+    [Clean.eclean Clean.sclean Clean.eclean_functional Clean.sclean_functional
+     Clean.qclean Clean.rclean Clean.qclean_functional Clean.rclean_functional
+     Clean.clean_rename Clean.clean_substitute Clean.clean_substitute_clause_1
+     Clean.clean_rapply Clean.clean_rapply_clause_1
+     Clean.dest_rshift Clean.dest_rshift_clause_2 Clean.dest_rshift_clause_2_clause_1
+     Clean.mk_qsucc Clean.dest_var
+     Clean.dest_ren Clean.dest_ren_clause_3 Clean.dest_ren_clause_3_clause_1 
+     Clean.dest_ren_clause_4 Clean.dest_ren_clause_4_clause_1
+     Clean.nat_add
      ]).
 
 (** Reduction flags to unfold all (level 2 -> level 1) evaluation 
     functions (LevelTwo.v). *)
 Ltac2 red_flags_eval () : RedFlags.t :=
   red_flags:(beta iota delta   
-    [eeval seval eeval_functional seval_functional
-     reval qeval reval_functional qeval_functional
-     assign_qnat assign_ren assign_term assign_subst
-     List.nth (* TODO use something else than [Lisnth]. *)
+    [T.eeval T.seval T.eeval_functional T.seval_functional
+     T.reval T.qeval T.reval_functional T.qeval_functional
+     T.assign_qnat T.assign_ren T.assign_term T.assign_subst
+     T.list_nth
      ]).
-
-End Make.
 
 (*********************************************************************************)
 (** *** [rasimpl]. *)
